soundness.v
@@ -1,0 +1,122 @@
+Require Import main.
+Require Import Classes.EquivDec.
+Require Import List.
+Require Import Bool.
+Import ListNotations.
+
+(*Note: compile main.v before running this .v file *)
+
+(* Lemmas about functions within the rhs module          *)
+Section rhs_lemmas.
+(*the following lemma states that isEmpty won't return a value different from false or true *)
+  Lemma isEmpty_sound  :forall NT T, forall r:rhs.t T NT, rhs.isEmpty r = false \/ rhs.isEmpty r = true.
+    Proof.   
+    intros.
+    destruct rhs.isEmpty;auto.
+    Qed.
+End rhs_lemmas.
+
+(*Lemmas about the soundness of functions within the reg_grammar module        *)
+Section reg_grammar_lemmas.
+  Variable T NT : Type.
+  Context  `{EqDec T eq} `{EqDec NT eq}.
+  (*The following lemma states that a grammar returned by build_grammar shall has the start *)
+  (*symbol and the rules passed as the parameters.                                          *)
+    Lemma build_grammar_sound : forall nt:NT, forall rules:list (NT * rhs.t T NT), reg_grammar.build_grammar nt rules = {|
+      reg_grammar.start_symbol := nt;
+      reg_grammar.rules := rules |}.
+  Proof.
+  intros. unfold reg_grammar.build_grammar. reflexivity. Qed.
+
+  (*the following lemma states that the function step_rhs is sound                         *)
+  Lemma step_rhs_sound : forall t:T, forall rhs: rhs.t T NT, reg_grammar.step_rhs t rhs = [] \/
+  reg_grammar.step_rhs t rhs = [None] \/ (exists nt, reg_grammar.step_rhs t rhs = [Some nt]).
+  Proof.
+  intros t rhs.
+  destruct rhs; auto.
+  simpl. destruct equiv_dec. auto.
+  auto.
+  simpl. destruct equiv_dec eqn:I;auto. 
+  right. right. exists (n). reflexivity.
+  Qed.
+
+  (*The following lemma states the soundness of the step_nt function. *)
+  Lemma step_nt_sound : forall rules,forall t, forall nt, reg_grammar.step_nt rules t nt =  [] \/
+  In None (reg_grammar.step_nt rules t nt)  \/ (exists n:NT, In (Some n) (reg_grammar.step_nt rules t nt)).
+  Proof.
+  intros.
+  destruct reg_grammar.step_nt.
+  - left. reflexivity.
+  - destruct o. right. right. simpl. exists n. left. reflexivity.
+    right. left. simpl. left. reflexivity. Qed.
+
+  (*The following lemma states the soundness of the step function *)
+  Definition step_sound: forall rules, forall t, forall acc, reg_grammar.step rules t acc = [] \/
+  In (None) (reg_grammar.step rules t acc) \/ (exists nt:NT, In (Some nt)(reg_grammar.step rules t acc)).
+  Proof.
+  intros.
+  destruct reg_grammar.step.
+  - left. reflexivity.
+  - destruct o. right. right. exists n. simpl. left. reflexivity.
+    right. left. simpl. left. reflexivity.
+  Qed.
+
+  (*The following lemmas states the soundness of the parse' function, the main parser loop.*)
+  (*By the definition of parse', it should return or a empty list, or a list that has None *)
+  (*or a list that contains Some nt in it, some NT being a nonterminal symbol              *)
+  Definition parse'_sound: forall rules, forall lt, forall lnt, reg_grammar.parse' rules lt lnt = [] 
+  \/ In (None) (reg_grammar.parse' rules lt lnt) \/ (exists nt:NT, In (Some nt) (reg_grammar.parse' rules lt lnt)).
+  Proof.
+  intros.
+  destruct reg_grammar.parse'.
+  - left. reflexivity.
+  - destruct o. right. right. exists n. simpl. left. reflexivity.
+    right. left. simpl. left. reflexivity.
+  Qed.
+
+  Lemma parse'_app_nil : forall g l acc, acc |> reg_grammar.parse' g (l ++ []) = acc 
+  |> reg_grammar.parse' g l \/ acc |> reg_grammar.parse' g ([]++ l) = acc |> reg_grammar.parse' g l.
+  Proof.
+  induction l; simpl;auto.
+  Qed.
+  Lemma parse'_nil :
+    forall g l ,
+      reg_grammar.parse' g l [] = [].
+  Proof.
+    induction l; simpl; auto.
+  Qed.
+  Lemma parse'_app :
+    forall g l1 l2 acc,
+      acc |> reg_grammar.parse' g (l1 ++ l2) =
+      acc |> reg_grammar.parse' g l1 |> reg_grammar.parse' g l2.
+  Proof.
+    induction l1; simpl; auto.
+  Qed.
+
+  (*The following lemma state that the is_final function may always return true or false*)
+  Lemma is_final_sound : forall r:list (NT * rhs.t T NT),forall l:list (option NT), reg_grammar.is_final r l = true \/ 
+  reg_grammar.is_final r l = false.
+ Proof.
+    intros r l.
+    destruct reg_grammar.is_final;auto.
+  Qed.
+
+  (*The following lemmas states properties about the soundness of the grammar parser *)
+  (*falta coisa*)
+  Lemma parse_companion : forall grammar, forall l, reg_grammar.parse grammar l = true \/ 
+  reg_grammar.parse grammar l = false.
+  Proof.
+  intros.
+  destruct reg_grammar.parse;auto.
+  Qed.
+End reg_grammar_lemmas.
+
+Section dfa_lemmas.
+  Variable (S A : Type).
+  (*The following lemma asserts that a is_final function should always return true or false *)
+  Lemma run_companion : forall m:dfa.t S A, forall l, dfa.run m l = true \/ dfa.run m l = false.
+    Proof.
+    intros.
+    destruct dfa.run;auto.
+    Qed.
+End dfa_lemmas.
